LeanHttp.lean
@@ -1,4 +1,7 @@
 import LeanHttp.Types
+import LeanHttp.Version
+import LeanHttp.Request
+import LeanHttp.Syntax
 import LeanHttp.Error
 import LeanHttp.Headers
 import LeanHttp.Session
